Lp2lc/Active/Util.lean
@@ -4,37 +4,31 @@ import «Lp2lc».Active.Shared
 
 namespace Lp2lc.Active.Util
 
+/-- Universe-1 carrier for PHOAS indices. -/
+abbrev Index := Type
+
+class FBound (I : Index) (K : Index -> Type) where -- fixed-point cast, looks like a reversed Env, it cast `Trm I` into something Val.depFn can accept
+  fwd : K I -> I -- useful in eval, definition uses the inverse but interpreter is not allowed to see it.
+  rev : I -> K I
+  fwdRoundtrip : (value : K I) -> rev (fwd value) = value
+
+attribute [simp] FBound.fwdRoundtrip
+
+inductive Outcome (T : Index)
+| some (v: T)
+| error
+| outOfFuel
+
+namespace Outcome
+
+def isSome : (self: Outcome T) -> Prop
+| .some _ => true
+| _ => false
+
+end Outcome
 
 def ByteCode := String
 
 abbrev Name := String
-
-section
-
-variable {Key : Type} {V : Type}
-
-abbrev Lookup := Key → Option V
-
-namespace Lookup
-
-def empty : Lookup (Key := Key) (V := V) := fun _ => none
-
-def set [DecidableEq Key] (σ : Lookup (Key := Key) (V := V)) (x : Key) (v : V) :
-    Lookup (Key := Key) (V := V) :=
-  fun y => if y = x then some v else σ y
-
-@[simp] theorem set_same [DecidableEq Key] (σ : Lookup (Key := Key) (V := V)) (x : Key)
-    (v : V) :
-  set σ x v x = some v := by
-  simp [set]
-
-@[simp] theorem set_other [DecidableEq Key] (σ : Lookup (Key := Key) (V := V)) (x y : Key)
-    (v : V) (h : y ≠ x) :
-  set σ x v y = σ y := by
-  simp [set, h]
-
-end Lookup
-
-end
 
 end Util
