Lp2lc/Active/DTLC/Runtime.lean
@@ -1,0 +1,9 @@
+import «Lp2lc».Active.DTLC.Proof
+
+namespace Lp2lc.Active
+
+namespace DTLC
+
+end DTLC
+
+end Lp2lc.Active
