Lp2lc/Experiments/Util.lean
@@ -1,0 +1,35 @@
+
+
+import «Lp2lc».Active.Shared
+
+namespace Lp2lc.Active.Util
+
+section
+
+variable {Key : Type} {V : Type}
+
+abbrev Lookup := Key → Option V
+
+namespace Lookup
+
+def empty : Lookup (Key := Key) (V := V) := fun _ => none
+
+def set [DecidableEq Key] (σ : Lookup (Key := Key) (V := V)) (x : Key) (v : V) :
+    Lookup (Key := Key) (V := V) :=
+  fun y => if y = x then some v else σ y
+
+@[simp] theorem set_same [DecidableEq Key] (σ : Lookup (Key := Key) (V := V)) (x : Key)
+    (v : V) :
+  set σ x v x = some v := by
+  simp [set]
+
+@[simp] theorem set_other [DecidableEq Key] (σ : Lookup (Key := Key) (V := V)) (x y : Key)
+    (v : V) (h : y ≠ x) :
+  set σ x v y = σ y := by
+  simp [set, h]
+
+end Lookup
+
+end
+
+end Util
